Added Hoare triples for all of the semantic commands, strutural rules, the read command, and method calls.

Java/src/Semantics/OperationalSemantics.v
@@ -1,6 +1,6 @@
 Require Import Program SepAlg AssertionLogic SpecLogic SepAlgMap.
 Require Import MapInterface MapFacts.
-Require Import ILInsts ILogic ILEmbed Open Subst Stack Lang.
+Require Import ILInsts ILogic ILEmbed Open Subst Stack Lang SemCmd.
 
 Import SepAlgNotations.
 
@@ -8,178 +8,6 @@ Set Implicit Arguments.
 Unset Strict Implicit.
 
 Section Commands.
-
-  Definition semCmdType := Prog_wf -> nat -> stack -> heap -> option (stack * heap) -> Prop.
-  Definition safe (c : semCmdType) P s t n := ~(c P s t n None).
-  Definition frame_property (c : semCmdType) :=
-    forall P s s' (big big' frame h : heap) n
-      (HFrame : sa_mul h frame big)
-      (HSafe  : forall m, m <= n -> safe c P m s h)
-      (HSem   : c P n s big (Some (s', big'))),
-      exists h', sa_mul h' frame big' /\ c P n s h (Some (s', h')).
-
-  Record semCmd := {
-    cmd_rel   :> Prog_wf -> nat -> stack -> heap -> option (stack * heap) -> Prop;
-    cmd_zero  :  forall P s h cfg, ~(cmd_rel P 0 s h cfg);
-    cmd_frame :  frame_property cmd_rel
-  }.
-
-  Definition not_modifies (c : semCmdType) x : Prop :=
-    forall P s s' h h' n (HSem : c P n s h (Some (s', h'))),
-      s x = s' x.
-
-  Lemma safe_zero : forall (c : semCmd) P s t, safe c P 0 s t.
-  Proof.
-    intros; apply cmd_zero.
-  Qed.
-
-  Global Opaque sa_mul.
-
-  Implicit Arguments Build_semCmd [].
-
-  Program Definition later_cmd (c : semCmd) : semCmd := Build_semCmd
-    (fun P n => match n return stack -> heap -> option (stack * heap) -> Prop with
-                  | O => fun _ _ _ => False
-                  | S n => c P n end) _ _.
-  Next Obligation.
-    unfold frame_property; intros.
-    destruct n as [| n]; unfold safe in HSafe; simpl in *; [contradiction |].
-    eapply cmd_frame; eauto. 
-    intros m HLe HFail; apply (HSafe (S m)); auto with arith.
-  Qed.
-
-  (* Skip *)
-
-  Inductive skip_sem : semCmdType :=
-  | s_ok : forall P s h, skip_sem P 1 s h (Some (s, h)).
-  Program Definition skip_cmd := @Build_semCmd skip_sem _ _.
-  Next Obligation.
-    intros H. inversion H.
-  Qed.
-  Next Obligation.
-    unfold frame_property; intros.
-    inversion HSem; subst; clear HSem.
-    exists h; auto using skip_sem.
-  Qed.
-
-  (* Seq *)
-  Inductive seq_sem (c1 c2 : semCmd) : semCmdType :=
-  | seq_failL : forall P n s h,
-      c1 P n s h None ->
-      seq_sem c1 c2 P (S n) s h None
-  | seq_failR : forall P n n' s s' h h',
-      c1 P n s h (Some (s', h')) ->
-      c2 P n' s' h' None ->
-      seq_sem c1 c2 P (S (n + n')) s h None
-  | seq_ok    : forall P n n0 s s0 s1 h h0 h1,
-      c1 P n  s  h  (Some (s0, h0)) ->
-      c2 P n0 s0 h0 (Some (s1, h1)) ->
-      seq_sem c1 c2 P (S (n + n0)) s h (Some (s1, h1)).
-  Program Definition seq_cmd c1 c2 := @Build_semCmd (seq_sem c1 c2) _ _.
-  Next Obligation.
-    intros H; inversion H.
-  Qed.
-  Next Obligation with eauto using seq_sem.
-    unfold frame_property; intros.
-    inversion HSem; subst; clear HSem.
-    edestruct (@cmd_frame c1) as [h0 [HFrame0 HSem0]]...
-    + intros m HLe HFail; apply HSafe with (S m); [omega | ]...
-    + edestruct (@cmd_frame c2) as [hr [HFrame1 HSem1]]...
-      intros m HLe HFail; apply HSafe with (S (n0 + m)); [omega | ]...
-  Qed.
-
-  (* Nondet *)
-  Inductive nondet_sem (c1 c2 : semCmd) : semCmdType :=
-  | nondet_failL : forall P n s h,
-      c1 P n s h None ->
-      nondet_sem c1 c2 P (S n) s h None
-  | nondet_okL   : forall P n s s' h h',
-      c1 P n s h (Some (s', h')) ->
-      nondet_sem c1 c2 P (S n) s h (Some (s', h'))
-  | nondet_failR : forall P n s h,
-      c2 P n s h None ->
-      nondet_sem c1 c2 P (S n) s h None
-  | nondet_okR   : forall P n s s' h h',
-      c2 P n s h (Some (s', h')) ->
-      nondet_sem c1 c2 P (S n) s h (Some (s', h')).
-  Program Definition nondet_cmd c1 c2 := @Build_semCmd (nondet_sem c1 c2) _ _.
-  Next Obligation.
-    intros H; inversion H.
-  Qed.
-  Next Obligation with eauto using nondet_sem.
-    unfold frame_property; intros.
-    inversion HSem; subst; clear HSem.
-    + edestruct (@cmd_frame c1) as [h0 [HFrame0 HSem0]]...
-      intros m HLe HFail; apply HSafe with (S m); [omega |]...
-    + edestruct (@cmd_frame c2) as [h0 [HFrame0 HSem0]]...
-      intros m HLe HFail; apply HSafe with (S m); [omega |]...
-  Qed.
-
-  (* Kleene star *)
-  Inductive kleene_sem (c : semCmd) : semCmdType :=
-  | kleene_emp       : forall P s h,
-      kleene_sem c P 1 s h (Some (s, h))
-  | kleene_fail_one  : forall P n s h,
-      c P n s h None ->
-      kleene_sem c P (S n) s h None
-  | kleene_fail_many : forall P n n0 s s0 h h0,
-      c P n s h (Some (s0, h0)) ->
-      kleene_sem c P n0 s0 h0 None ->
-      kleene_sem c P (S (n + n0)) s h None
-  | kleene_step_ok   : forall P n n0 s s0 s1 h h0 h1,
-      c P n s h (Some (s0, h0)) ->
-      kleene_sem c P n0 s0 h0 (Some (s1, h1)) ->
-      kleene_sem c P (S (n + n0)) s h (Some (s1, h1)).
-  Program Definition kleene_cmd c := @Build_semCmd (kleene_sem c) _ _.
-  Next Obligation.
-    intros H; inversion H.
-  Qed.
-  Next Obligation with eauto using kleene_sem.
-    unfold frame_property; intros.
-    generalize dependent h; remember (Some (s', big')) as cfg; induction HSem;
-      inversion Heqcfg; subst; intros; clear Heqcfg...
-    edestruct (@cmd_frame c) as [h' [HFrame0 HSem0]]...
-    + intros m HLe HFail; apply HSafe with (S m); [omega |]...
-    + destruct (IHHSem (eq_refl _) h' HFrame0) as [hr [HFrame1 HSem1]]...
-      intros m HLe HFail; apply HSafe with (S (n + m)); [omega |]...
-  Qed.
-
-  (* TODO: update the description
-     assume command -- this command is a bit of a hack that just skips if
-     a check holds and loops otherwise, this way allowing to encode if/while
-     using nondeterministic choice/Kleene star *)
-  Inductive assume_sem (e : dexpr) : semCmdType :=
-  | assume_ok : forall P s h, eval e s = vbool true -> assume_sem e P 1 s h (Some (s, h)).
-  Program Definition assume_cmd P := @Build_semCmd (assume_sem P) _ _.
-  Next Obligation.
-    intros H; inversion H.
-  Qed.
-  Next Obligation.
-    unfold frame_property; simpl; intros.
-    remember (Some (s', big')) as cfg; induction HSem.
-    inversion Heqcfg; subst; eauto using assume_sem.
-  Qed.
-
-  Lemma assume_inv P e n s s0 h h0 (HSem : assume_cmd e P n s h (Some (s0, h0))) : 
-      s = s0 /\ h = h0.
-  Proof.  
-    intros; remember (Some (s0, h0)); induction HSem; subst;
-    try inversion Heqo; intuition.
-  Qed.
-
-  Inductive assert_sem (e : dexpr) : semCmdType :=
-  | assert_ok   : forall P s h (HP : eval e s = vbool true),
-    assert_sem e P 1 s h (Some (s, h))
-  | assert_fail : forall P s h (HNP : eval e s = vbool false),
-    assert_sem e P 1 s h None.
-  Program Definition assert_cmd e := @Build_semCmd (assert_sem e) _ _.
-  Next Obligation.
-    intros H; inversion H.
-  Qed.
-  Next Obligation.
-    unfold frame_property; simpl; intros.
-    inversion HSem; subst; eauto using assert_sem.
-  Qed.  
 
   Inductive assign_sem (x : var) (e : dexpr) : semCmdType :=
   | assign_ok : forall P s h v
@@ -333,12 +161,12 @@ Section Commands.
       (HL : semantics cl scl)
       (HR : semantics cr scr),
       semantics (cif e cl cr) (nondet_cmd
-        (seq_cmd (assume_cmd e) scl)
-        (seq_cmd (assume_cmd (E_not e)) scr))
+        (seq_cmd (assume_cmd (pure_eval e)) scl)
+        (seq_cmd (assume_cmd (pure_eval (E_not e))) scr))
   | semwhile  : forall e c sc
       (HS : semantics c sc),
       semantics (cwhile e c) (seq_cmd (kleene_cmd
-        (seq_cmd (assume_cmd e) sc)) (assume_cmd (E_not e)))
+        (seq_cmd (assume_cmd (pure_eval e)) sc)) (assume_cmd (pure_eval (E_not e))))
   | semdcall  : forall (x y : var) m es c sc 
       (HSem     : semantics c sc),
       semantics (cdcall x y m es) (call_cmd x ((liftn val_class) (var_expr y)) m ((E_var y) :: es) c sc)
@@ -346,7 +174,7 @@ Section Commands.
       (HSem     : semantics c sc),
       semantics (cscall x C m es) (call_cmd x (open_const C) m es c sc)
   | semassert : forall e,
-      semantics (cassert e) (assert_cmd e).
+      semantics (cassert e) (assert_cmd (pure_eval e)).
 
   Definition c_not_modifies c x :=
     forall sc, semantics c sc -> not_modifies sc x.
@@ -414,45 +242,11 @@ Section Commands.
 
 End Commands.
 
-  Program Definition triple_aux (p q : sasn) (c : semCmd) : spec :=
-    mk_spec (fun n P => forall P' m k s h, Prog_wf_sub P P' -> m <= n -> k <= m -> 
-                                           p s P' m h ->
-      safe c P' k s h /\
-      forall h' s', c P' k s h (Some (s', h')) -> (q s' P' (m - k) h')) _ _.
-  Next Obligation.
-    apply H0; try eassumption.
-    etransitivity; eassumption.
-  Qed.
-
   Local Transparent ILPre_Ops.
   Local Transparent ILFun_Ops.
 
-  Add Parametric Morphism : triple_aux with signature
-    lentails --> lentails ++> eq ==> lentails
-    as triple_aux_entails_m.
-  Proof.
-    intros p p' Hp q q' Hq c n t H P m k s h HP Hmn Hkm Hp'.
-    apply Hp in Hp'; try apply _.    
-    simpl in *.
-    specialize (H _ _ _ _ _ HP Hmn Hkm Hp').
-    destruct H as [Hsafe H].
-    split; [assumption|].
-    intros h' s' Hc.
-    apply Hq.
-    apply H. assumption.
-  Qed.
-
-  Add Parametric Morphism : triple_aux with signature
-    lequiv ==> lequiv ==> eq ==> lequiv
-    as triple_aux_lequiv_m.
-  Proof.
-    split.
-    + rewrite H, H0; reflexivity.
-    + rewrite <- H, <- H0; reflexivity.
-  Qed.
-
   Definition triple (P Q : sasn) (c : cmd) :=
-    Forall sc : semCmd, (semantics c sc) ->> triple_aux P Q sc.
+    Forall sc : semCmd, (semantics c sc) ->> {{P}} sc {{Q}}.
 
   Notation " '{[' P ']}' c '{[' Q ']}' " := (triple P Q c) (at level 89,
     format " {[ P ]} '/' c '/' {[ Q ]} ").
@@ -473,7 +267,7 @@ Open Scope open_scope.
     (method_spec C m ps r P Q) (at level 60).
 
   Lemma c_triple_zero P (p q : sasn) (c : cmd) :
-    ({[ p ]} c {[ q ]}) 0 P.
+    ({[ p ]} c {[ q ]}) P 0.
   Proof.
     intros sc n Hn Q HPQ sem R k m s h HQR Hk Hv Hp.
     assert (m = 0) by omega.
